FullVersioned

BlockCacheSystem/BlockCache.i.dfy
@@ -2,14 +2,12 @@ include "../Betree/Betree.i.dfy"
 include "../lib/Base/sequences.i.dfy"
 include "../lib/Base/Maps.s.dfy"
 include "../Betree/Graph.i.dfy"
-include "../BlockCacheSystem/AsyncSectorDiskModel.i.dfy"
+include "../BlockCacheSystem/BlockDisk.i.dfy"
 include "../PivotBetree/PivotBetreeSpec.i.dfy"
-include "JournalRange.i.dfy"
-include "JournalInterval.i.dfy"
 
 //
 // A BlockCache implements the BlockInterface by caching over an
-// AsyncSectorDisk. At this layer, the disk provides high-level sectors
+// BlockDisk. At this layer, the disk provides high-level sectors
 // (containing either this module's indirection tables or the Node
 // type of the application, a not-yet-bound parameter).
 //
@@ -23,12 +21,9 @@ module BlockCache refines Transactable {
   import opened Options
   import opened NativeTypes
   import opened DiskLayout
-  import opened Journal
-  import opened JournalRanges
-  import opened JournalIntervals
   import opened SectorType
 
-  import Disk = AsyncSectorDisk
+  import Disk = BlockDisk
 
   type ReqId = Disk.ReqId
   datatype Constants = Constants()
@@ -39,14 +34,6 @@ module BlockCache refines Transactable {
 
   datatype OutstandingWrite = OutstandingWrite(ref: Reference, loc: Location)
   datatype OutstandingRead = OutstandingRead(ref: Reference)
-  //datatype OutstandingJournalWrite = OutstandingJournalWrite(index: int)
-
-  datatype SyncReqStatus = State1 | State2 | State3
-
-  datatype SuperblockReadResult =
-      | SuperblockSuccess(value: Superblock)
-      | SuperblockUnfinished
-      | SuperblockCorruption
 
   datatype Variables =
     | Ready(
@@ -54,54 +41,22 @@ module BlockCache refines Transactable {
         frozenIndirectionTable: Option<IndirectionTable>,
         ephemeralIndirectionTable: IndirectionTable,
 
-        outstandingIndirectionTableWrite: Option<ReqId>,
+        persistentIndirectionTableLoc: Location,
         frozenIndirectionTableLoc: Option<Location>,
-        frozenJournalPosition: int,
 
-        superblockWrite: Option<ReqId>,
-
+        outstandingIndirectionTableWrite: Option<ReqId>,
         outstandingBlockWrites: map<ReqId, OutstandingWrite>,
         outstandingBlockReads: map<ReqId, OutstandingRead>,
 
-        inMemoryJournalFrozen: seq<JournalEntry>,
-        inMemoryJournal: seq<JournalEntry>,
-        outstandingJournalWrites: set<ReqId>,
-        writtenJournalLen: int,
-
-        replayJournal: seq<JournalEntry>,
-
-        superblock: Superblock,
-        whichSuperblock: int,
-        newSuperblock: Option<Superblock>,
-
-        cache: map<Reference, Node>,
-
-        syncReqs: map<uint64, SyncReqStatus>
+        cache: map<Reference, Node>
       )
 
-    | LoadingOther(
-        superblock: Superblock,
-        whichSuperblock: int,
-
-        indirectionTableRead: Option<ReqId>,
-        journalFrontRead: Option<ReqId>,
-        journalBackRead: Option<ReqId>,
-
-        indirectionTable: Option<IndirectionTable>,
-        journalFront: Option<JournalRange>,
-        journalBack: Option<JournalRange>,
-
-        syncReqs: map<uint64, SyncReqStatus>
+    | LoadingIndirectionTable(
+        indirectionTableLoc: Location,
+        indirectionTableRead: Option<ReqId>
       )
 
-    | LoadingSuperblock(
-        outstandingSuperblock1Read: Option<ReqId>,
-        outstandingSuperblock2Read: Option<ReqId>,
-        superblock1: SuperblockReadResult,
-        superblock2: SuperblockReadResult,
-
-        syncReqs: map<uint64, SyncReqStatus>
-      )
+    | Unready
 
   predicate IsAllocated(s: Variables, ref: Reference)
   requires s.Ready?
@@ -150,106 +105,21 @@ module BlockCache refines Transactable {
         s.outstandingBlockWrites[id].loc.addr != loc.addr)
   }
 
-  function IncrementSuperblockCounter(i: uint64) : uint64
-  {
-    if i == 0xffff_ffff_ffff_ffff then
-      0
-    else
-      i + 1
-  }
-
-  predicate increments1(i: uint64, j: uint64) {
-    j == IncrementSuperblockCounter(i)
-  }
-
-  function SelectSuperblockIndex(
-      superblock1: Superblock, 
-      superblock2: Superblock) : int
-  {
-    if increments1(superblock1.counter, superblock2.counter) then
-      1
-    else
-      0
-  }
-
-  function SelectSuperblock(
-      superblock1: Superblock, 
-      superblock2: Superblock) : Superblock
-  {
-    if SelectSuperblockIndex(superblock1, superblock2) == 1 then
-      superblock2
-    else
-      superblock1
-  }
-
-  function syncReqs3to2(syncReqs: map<uint64, SyncReqStatus>) : map<uint64, SyncReqStatus>
-  {
-    map id | id in syncReqs :: (if syncReqs[id] == State3 then State2 else syncReqs[id])
-  }
-
-  function syncReqs2to1(syncReqs: map<uint64, SyncReqStatus>) : map<uint64, SyncReqStatus>
-  {
-    map id | id in syncReqs :: (if syncReqs[id] == State2 then State1 else syncReqs[id])
-  }
-
-  // Journal is written in a circular array, so to load the log
-  // we may have to read back two chunks.
-
-  function JournalFrontIntervalOfSuperblock(superblock: Superblock) : Option<JournalInterval>
-  requires superblock.journalStart < NumJournalBlocks()
-  {
-    JournalFrontInterval(
-      superblock.journalStart as int,
-      superblock.journalLen as int)
-  }
-
-  function JournalBackIntervalOfSuperblock(superblock: Superblock) : Option<JournalInterval>
-  requires superblock.journalStart < NumJournalBlocks()
-  requires superblock.journalLen <= NumJournalBlocks()
-  {
-    JournalBackInterval(
-      superblock.journalStart as int,
-      superblock.journalLen as int)
-  }
-
-  predicate WFSuperblock(superblock: Superblock)
-  {
-    && superblock.journalStart < NumJournalBlocks()
-    && superblock.journalLen <= NumJournalBlocks()
-    && ValidIndirectionTableLocation(superblock.indirectionTableLoc)
-  }
-
-  datatype JournalStep =
-      | JSNew(entries: seq<JournalEntry>)
-      | JSReplay(entries: seq<JournalEntry>)
-
   datatype Step =
-    | WriteBackReqStep(ref: Reference)
-    | WriteBackRespStep
+    | WriteBackNodeReqStep(ref: Reference)
+    | WriteBackNodeRespStep
     | WriteBackIndirectionTableReqStep
     | WriteBackIndirectionTableRespStep
-    | WriteBackJournalReqStep(jr: JournalRange)
-    | WriteBackJournalRespStep
-    | WriteBackSuperblockReq_Basic_Step
-    | WriteBackSuperblockReq_UpdateIndirectionTable_Step
-    | WriteBackSuperblockRespStep
     | UnallocStep(ref: Reference)
     | PageInReqStep(ref: Reference)
     | PageInRespStep
     | PageInIndirectionTableReqStep
     | PageInIndirectionTableRespStep
-    | PageInJournalReqStep(which: int)
-    | PageInJournalRespStep(which: int)
-    | PageInSuperblockReqStep(which: int)
-    | PageInSuperblockRespStep(which: int)
-    | FinishLoadingSuperblockPhaseStep
-    | FinishLoadingOtherPhaseStep
+    | ReceiveLocStep
     | EvictStep(ref: Reference)
     | FreezeStep
-    | PushSyncReqStep(id: uint64)
-    | PopSyncReqStep(id: uint64)
     | NoOpStep
-    | TransactionStep(ops: seq<Op>, journalStep: JournalStep)
+    | TransactionStep(ops: seq<Op>)
 
   function assignRefToLocation(indirectionTable: IndirectionTable, ref: Reference, loc: Location) : IndirectionTable
   {
@@ -264,7 +134,7 @@ module BlockCache refines Transactable {
     forall reqId | reqId in outstandingBlockReads :: outstandingBlockReads[reqId].ref != ref
   }
 
-  predicate WriteBackReq(k: Constants, s: Variables, s': Variables, dop: DiskOp, ref: Reference)
+  predicate WriteBackNodeReq(k: Constants, s: Variables, s': Variables, dop: DiskOp, ref: Reference)
   {
     && dop.ReqWriteNodeOp?
     && s.Ready?
@@ -290,21 +160,11 @@ module BlockCache refines Transactable {
     && s'.outstandingBlockWrites == s.outstandingBlockWrites[dop.id := OutstandingWrite(ref, dop.reqWriteNode.loc)]
     && s'.outstandingBlockReads == s.outstandingBlockReads
     && s'.outstandingIndirectionTableWrite == s.outstandingIndirectionTableWrite
-    && s'.syncReqs == s.syncReqs
     && s'.frozenIndirectionTableLoc == s.frozenIndirectionTableLoc
-    && s'.frozenJournalPosition == s.frozenJournalPosition
-    && s'.superblockWrite == s.superblockWrite
-    && s'.inMemoryJournal == s.inMemoryJournal
-    && s'.inMemoryJournalFrozen == s.inMemoryJournalFrozen
-    && s'.outstandingJournalWrites == s.outstandingJournalWrites
-    && s'.writtenJournalLen == s.writtenJournalLen
-    && s'.replayJournal == s.replayJournal
-    && s'.superblock == s.superblock
-    && s'.whichSuperblock == s.whichSuperblock
-    && s'.newSuperblock == s.newSuperblock
+    && s'.persistentIndirectionTableLoc == s.persistentIndirectionTableLoc
   }
 
-  predicate WriteBackResp(k: Constants, s: Variables, s': Variables, dop: DiskOp)
+  predicate WriteBackNodeResp(k: Constants, s: Variables, s': Variables, dop: DiskOp)
   {
     && dop.RespWriteNodeOp?
     && s.Ready?
@@ -319,14 +179,12 @@ module BlockCache refines Transactable {
     && s.frozenIndirectionTable.Some?
     && var loc := dop.reqWriteIndirectionTable.loc;
     && ValidIndirectionTableLocation(loc)
-    && s.newSuperblock.None?
-    && !overlap(
-          loc,
-          s.superblock.indirectionTableLoc)
     && dop.reqWriteIndirectionTable.indirectionTable == s.frozenIndirectionTable.value
     && s.frozenIndirectionTable.value.graph.Keys <= s.frozenIndirectionTable.value.locs.Keys
     && s.outstandingIndirectionTableWrite.None?
-    //&& s.outstandingBlockWrites == map[]
+    && !overlap(
+          loc,
+          s.persistentIndirectionTableLoc)
     && s' == s
       .(outstandingIndirectionTableWrite := Some(dop.id))
       .(frozenIndirectionTableLoc := Some(loc))
@@ -338,149 +196,6 @@ module BlockCache refines Transactable {
     && s.Ready?
     && s.outstandingIndirectionTableWrite == Some(dop.id)
     && s' == s.(outstandingIndirectionTableWrite := None)
-  }
-
-  predicate WriteBackJournalReq(k: Constants, s: Variables, s': Variables, dop: DiskOp, jr: JournalRange)
-  {
-    && s.Ready?
-
-    && var j :=
-        if s.inMemoryJournalFrozen == [] then
-          s.inMemoryJournal
-        else
-          s.inMemoryJournalFrozen;
-
-    && JournalRangeParses(jr, j)
-    && JournalRangeLen(jr) + s.writtenJournalLen <= NumJournalBlocks() as int
-    && JournalRangeLen(jr) > 0
-    && s.superblockWrite.None?
-    && s.superblock.journalStart < NumJournalBlocks()
-    && 0 <= s.writtenJournalLen <= NumJournalBlocks() as int
-    && var startPos := JournalPosAdd(
-        s.superblock.journalStart as int,
-        s.writtenJournalLen);
-
-    && var writtenJournalLen' :=
-        s.writtenJournalLen + JournalRangeLen(jr);
-
-    && var frozenJournalPosition' := 
-        if s.inMemoryJournalFrozen == [] then
-          s.frozenJournalPosition
-        else
-          writtenJournalLen';
-
-    && var inMemoryJournal' :=
-        if s.inMemoryJournalFrozen == [] then
-          []
-        else
-          s.inMemoryJournal;
-
-    && var syncReqs' :=
-        if s.inMemoryJournalFrozen == [] then
-          syncReqs3to2(s.syncReqs)
-        else
-          s.syncReqs;
-
-    && var inMemoryJournalFrozen' := [];
-
-    && dop.ReqWriteJournalOp?
-    && dop.reqWriteJournal.journal == jr
-    && dop.reqWriteJournal.start == startPos
-    && s' == s
-        .(outstandingJournalWrites := s.outstandingJournalWrites + {dop.id})
-        .(writtenJournalLen := writtenJournalLen')
-        .(frozenJournalPosition := frozenJournalPosition')
-        .(inMemoryJournal := inMemoryJournal')
-        .(inMemoryJournalFrozen := inMemoryJournalFrozen')
-        .(syncReqs := syncReqs')
-  }
-
-  predicate WriteBackJournalResp(k: Constants, s: Variables, s': Variables, dop: DiskOp)
-  {
-    && s.Ready?
-    && dop.RespWriteJournalOp?
-    && dop.id in s.outstandingJournalWrites
-    && s' == s
-       .(outstandingJournalWrites := s.outstandingJournalWrites - {dop.id})
-  }
-
-  predicate WriteBackSuperblockReq_Basic(k: Constants, s: Variables, s': Variables, dop: DiskOp)
-  {
-    && s.Ready?
-    && dop.ReqWriteSuperblockOp?
-    && s.superblockWrite.None?
-    && s.outstandingJournalWrites == {}
-    && s.inMemoryJournalFrozen == []
-    && dop.which == (if s.whichSuperblock == 0 then 1 else 0)
-    && 0 <= s.writtenJournalLen <= NumJournalBlocks() as int
-    && var newSuperblock := Superblock(
-      IncrementSuperblockCounter(s.superblock.counter),
-      s.superblock.journalStart,
-      s.writtenJournalLen as uint64,
-      s.superblock.indirectionTableLoc
-    );
-    && dop.reqWriteSuperblock.superblock == newSuperblock
-    && s' == s
-        .(newSuperblock := Some(newSuperblock))
-        .(superblockWrite := Some(dop.id))
-  }
-
-  predicate WriteBackSuperblockReq_UpdateIndirectionTable(k: Constants, s: Variables, s': Variables, dop: DiskOp)
-  {
-    && s.Ready?
-    && dop.ReqWriteSuperblockOp?
-    && s.frozenIndirectionTableLoc.Some?
-    && s.outstandingIndirectionTableWrite.None?
-    && s.superblockWrite.None?
-    && s.outstandingBlockWrites == map[]
-    && s.outstandingJournalWrites == {}
-    && dop.which == (if s.whichSuperblock == 0 then 1 else 0)
-    && 0 <= s.superblock.journalStart < NumJournalBlocks()
-    && 0 <= s.frozenJournalPosition
-         <= s.writtenJournalLen
-         <= NumJournalBlocks() as int
-    && s.inMemoryJournalFrozen == []
-    && var newSuperblock := Superblock(
-      IncrementSuperblockCounter(s.superblock.counter),
-      JournalPosAdd(
-          s.superblock.journalStart as int,
-          s.frozenJournalPosition) as uint64,
-      (s.writtenJournalLen - s.frozenJournalPosition) as uint64,
-      s.frozenIndirectionTableLoc.value
-    );
-    && dop.reqWriteSuperblock.superblock == newSuperblock
-    && s' == s
-        .(newSuperblock := Some(newSuperblock))
-        .(superblockWrite := Some(dop.id))
-  }
-
-  predicate WriteBackSuperblockResp(k: Constants, s: Variables, s': Variables, dop: DiskOp)
-  {
-    && s.Ready?
-    && dop.RespWriteSuperblockOp?
-    && Some(dop.id) == s.superblockWrite
-    && s.newSuperblock.Some?
-    && s'.Ready?
-    && var isUpdatingTable :=
-        (s.newSuperblock.value.indirectionTableLoc != s.superblock.indirectionTableLoc);
-    && (isUpdatingTable ==> s.frozenIndirectionTable.Some?)
-    && s' == s.(superblockWrite := None)
-        .(superblock := s.newSuperblock.value)
-        .(newSuperblock := None)
-        .(whichSuperblock := if s.whichSuperblock == 0 then 1 else 0)
-        .(syncReqs := syncReqs2to1(s.syncReqs))
-        .(writtenJournalLen :=
-            if !isUpdatingTable then s.writtenJournalLen else
-                s.writtenJournalLen - s.frozenJournalPosition)
-        .(frozenJournalPosition :=
-            if !isUpdatingTable then s.frozenJournalPosition else 0)
-        .(frozenIndirectionTableLoc :=
-            if !isUpdatingTable then s.frozenIndirectionTableLoc else None)
-        .(frozenIndirectionTable :=
-            if !isUpdatingTable then s.frozenIndirectionTable else None)
-        .(persistentIndirectionTable :=
-            if !isUpdatingTable
-              then s.persistentIndirectionTable else s.frozenIndirectionTable.value)
   }
 
   predicate NoPredecessors(graph: map<Reference, seq<Reference>>, ref: Reference)
@@ -512,19 +227,9 @@ module BlockCache refines Transactable {
     && OutstandingBlockReadsDoesNotHaveRef(s.outstandingBlockReads, ref)
     && s'.outstandingBlockReads == s.outstandingBlockReads
     && s'.frozenIndirectionTable == s.frozenIndirectionTable
-    && s'.syncReqs == s.syncReqs
 
     && s'.frozenIndirectionTableLoc == s.frozenIndirectionTableLoc
-    && s'.frozenJournalPosition == s.frozenJournalPosition
-    && s'.superblockWrite == s.superblockWrite
-    && s'.inMemoryJournalFrozen == s.inMemoryJournalFrozen
-    && s'.inMemoryJournal == s.inMemoryJournal
-    && s'.outstandingJournalWrites == s.outstandingJournalWrites
-    && s'.writtenJournalLen == s.writtenJournalLen
-    && s'.replayJournal == s.replayJournal
-    && s'.superblock == s.superblock
-    && s'.whichSuperblock == s.whichSuperblock
-    && s'.newSuperblock == s.newSuperblock
+    && s'.persistentIndirectionTableLoc == s.persistentIndirectionTableLoc
   }
 
   predicate PageInReq(k: Constants, s: Variables, s': Variables, dop: DiskOp, ref: Reference)
@@ -557,190 +262,40 @@ module BlockCache refines Transactable {
   predicate PageInIndirectionTableReq(k: Constants, s: Variables, s': Variables, dop: DiskOp)
   {
     && dop.ReqReadIndirectionTableOp?
-    && s.LoadingOther?
+    && s.LoadingIndirectionTable?
 
     && s.indirectionTableRead.None?
-    && s.indirectionTable.None?
-    && dop.reqReadIndirectionTable.loc == s.superblock.indirectionTableLoc
     && s' == s.(indirectionTableRead := Some(dop.id))
   }
 
   predicate PageInIndirectionTableResp(k: Constants, s: Variables, s': Variables, dop: DiskOp)
   {
     && dop.RespReadIndirectionTableOp?
-    && s.LoadingOther?
+    && s.LoadingIndirectionTable?
     && dop.indirectionTable.Some?
     && WFCompleteIndirectionTable(dop.indirectionTable.value)
     && AllLocationsForDifferentRefsDontOverlap(dop.indirectionTable.value)
 
     && s.indirectionTableRead == Some(dop.id)
-    && s' == s
-        .(indirectionTableRead := None)
-        .(indirectionTable := Some(dop.indirectionTable.value))
-  }
-
-  predicate PageInJournalReq(k: Constants, s: Variables, s': Variables, dop: DiskOp, which: int)
-  {
-    && dop.ReqReadJournalOp?
-    && s.LoadingOther?
-    && (which == 0 || which == 1)
-    && s.superblock.journalStart < NumJournalBlocks()
-    && s.superblock.journalLen <= NumJournalBlocks()
-    && (which == 0 ==>
-      && JournalFrontIntervalOfSuperblock(s.superblock).Some?
-      && dop.reqReadJournal.interval
-          == JournalFrontIntervalOfSuperblock(s.superblock).value
-      && s.journalFrontRead.None?
-      && s.journalFront.None?
-      && s' == s.(journalFrontRead := Some(dop.id))
-    )
-    && (which == 1 ==>
-      && JournalBackIntervalOfSuperblock(s.superblock).Some?
-      && dop.reqReadJournal.interval
-          == JournalBackIntervalOfSuperblock(s.superblock).value
-      && s.journalBackRead.None?
-      && s.journalBack.None?
-      && s' == s.(journalBackRead := Some(dop.id))
-    )
-  }
-
-  predicate PageInJournalResp(k: Constants, s: Variables, s': Variables, dop: DiskOp, which: int)
-  {
-    && dop.RespReadJournalOp?
-    && s.LoadingOther?
-    && dop.journal.Some?
-    && (which == 0 || which == 1)
-    && (which == 0 ==>
-      && s.journalFrontRead == Some(dop.id)
-      && s' == s
-          .(journalFrontRead := None)
-          .(journalFront := Some(dop.journal.value))
-    )
-    && (which == 1 ==>
-      && s.journalBackRead == Some(dop.id)
-      && s' == s
-          .(journalBackRead := None)
-          .(journalBack := Some(dop.journal.value))
-    )
-  }
-
-  predicate PageInSuperblockReq(k: Constants, s: Variables, s': Variables, dop: DiskOp, which: int)
-  {
-    && dop.ReqReadSuperblockOp?
-    && s.LoadingSuperblock?
-    && dop.which == which
-    && (which == 0 || which == 1)
-    && (which == 0 ==> 
-      && s.outstandingSuperblock1Read.None?
-      && s.superblock1.SuperblockUnfinished?
-      && s' == s.(outstandingSuperblock1Read := Some(dop.id))
-    )
-    && (which == 1 ==> 
-      && s.outstandingSuperblock2Read.None?
-      && s.superblock2.SuperblockUnfinished?
-      && s' == s.(outstandingSuperblock2Read := Some(dop.id))
-    )
-  }
-
-  predicate PageInSuperblockResp(k: Constants, s: Variables, s': Variables, dop: DiskOp, which: int)
-  {
-    && dop.RespReadSuperblockOp?
-    && s.LoadingSuperblock?
-    && var sup := (
-        if dop.superblock.Some? &&
-            WFSuperblock(dop.superblock.value) then
-          SuperblockSuccess(dop.superblock.value)
-        else
-          SuperblockCorruption
-    );
-    && (which == 0 || which == 1)
-    && (which == 0 ==> 
-      && s.outstandingSuperblock1Read == Some(dop.id)
-      && s' == s
-          .(outstandingSuperblock1Read := None)
-          .(superblock1 := sup)
-    )
-    && (which == 1 ==> 
-      && s.outstandingSuperblock2Read == Some(dop.id)
-      && s' == s
-          .(outstandingSuperblock2Read := None)
-          .(superblock2 := sup)
-    )
-  }
-
-  predicate FinishLoadingSuperblockPhase(k: Constants, s: Variables, s': Variables, dop: DiskOp)
-  {
-    && dop.NoDiskOp?
-    && s.LoadingSuperblock?
-    // TODO account for case where one superblock or the other is corrupt
-    && s.superblock1.SuperblockSuccess?
-    && s.superblock2.SuperblockSuccess?
-    && (s.superblock1.SuperblockSuccess?
-        || s.superblock2.SuperblockSuccess?)
-    && (s.superblock1.SuperblockSuccess? && s.superblock2.SuperblockSuccess? ==>
-      s' == LoadingOther(
-        SelectSuperblock(s.superblock1.value, s.superblock2.value),
-        SelectSuperblockIndex(s.superblock1.value, s.superblock2.value),
-        None, None, None,
-        None, None, None,
-        s.syncReqs)
-    )
-    && (s.superblock1.SuperblockCorruption? ==>
-      s' == LoadingOther(
-        s.superblock2.value,
-        1,
-        None, None, None,
-        None, None, None,
-        s.syncReqs)
-    )
-    && (s.superblock2.SuperblockCorruption? ==>
-      s' == LoadingOther(
-        s.superblock1.value,
-        0,
-        None, None, None,
-        None, None, None,
-        s.syncReqs)
-    )
-  }
-
-  predicate FinishLoadingOtherPhase(k: Constants, s: Variables, s': Variables, dop: DiskOp)
-  {
-    && dop.NoDiskOp?
-    && s.LoadingOther?
-    && s.indirectionTable.Some?
-    && s.superblock.journalStart < NumJournalBlocks()
-    && s.superblock.journalLen <= NumJournalBlocks()
-    && (JournalFrontIntervalOfSuperblock(s.superblock).Some? ==> s.journalFront.Some?)
-    && (JournalBackIntervalOfSuperblock(s.superblock).Some? ==> s.journalBack.Some?)
-
-    && var fullRange := (
-        if JournalBackIntervalOfSuperblock(s.superblock).Some? then
-          JournalRangeConcat(s.journalFront.value, s.journalBack.value)
-        else if JournalFrontIntervalOfSuperblock(s.superblock).Some? then
-          s.journalFront.value
-        else
-          JournalRangeEmpty()
-    );
 
     && s'.Ready?
-    && s'.persistentIndirectionTable == s.indirectionTable.value
+    && s'.persistentIndirectionTable == dop.indirectionTable.value
     && s'.frozenIndirectionTable == None
-    && s'.ephemeralIndirectionTable == s.indirectionTable.value
-    && s'.outstandingIndirectionTableWrite == None
+    && s'.ephemeralIndirectionTable == dop.indirectionTable.value
+    && s'.persistentIndirectionTableLoc == s.indirectionTableLoc
     && s'.frozenIndirectionTableLoc == None
-    && s'.superblockWrite == None
+    && s'.outstandingIndirectionTableWrite == None
     && s'.outstandingBlockWrites == map[]
     && s'.outstandingBlockReads == map[]
-    && s'.inMemoryJournalFrozen == []
-    && s'.inMemoryJournal == []
-    && s'.outstandingJournalWrites == {}
-    && s'.writtenJournalLen == s.superblock.journalLen as int
-    && JournalRangeParses(fullRange, s'.replayJournal)
-    && s'.superblock == s.superblock
-    && s'.whichSuperblock == s.whichSuperblock
-    && s'.newSuperblock == None
     && s'.cache == map[]
-    && s'.syncReqs == s.syncReqs
+  }
+
+  predicate ReceiveLoc(k: Constants, s: Variables, s': Variables, dop: DiskOp)
+  {
+    && s.Unready?
+    && s'.LoadingIndirectionTable?
+    && s'.indirectionTableRead.None?
+    && ValidIndirectionTableLocation(s'.indirectionTableLoc)
   }
 
   predicate Evict(k: Constants, s: Variables, s': Variables, dop: DiskOp, ref: Reference)
@@ -762,30 +317,9 @@ module BlockCache refines Transactable {
     && s.Ready?
     && dop.NoDiskOp?
     && s.outstandingIndirectionTableWrite.None?
-    && s.superblockWrite.None?
-    && s.replayJournal == []
     && s' ==
         s.(frozenIndirectionTable := Some(s.ephemeralIndirectionTable))
          .(frozenIndirectionTableLoc := None)
-         .(inMemoryJournalFrozen := s.inMemoryJournalFrozen + s.inMemoryJournal)
-         .(inMemoryJournal := [])
-         .(frozenJournalPosition := s.writtenJournalLen)
-         .(syncReqs := syncReqs3to2(s.syncReqs))
-  }
-
-  predicate PushSyncReq(k: Constants, s: Variables, s': Variables, dop: DiskOp, id: uint64)
-  {
-    && dop.NoDiskOp?
-    && id !in s.syncReqs
-    && s' == s.(syncReqs := s.syncReqs[id := State3])
-  }
-
-  predicate PopSyncReq(k: Constants, s: Variables, s': Variables, dop: DiskOp, id: uint64)
-  {
-    && dop.NoDiskOp?
-    && id in s.syncReqs
-    && s.syncReqs[id] == State1
-    && s' == s.(syncReqs := MapRemove1(s.syncReqs, id))
   }
 
   predicate NoOp(k: Constants, s: Variables, s': Variables, dop: DiskOp)
@@ -793,30 +327,12 @@ module BlockCache refines Transactable {
     && (
       || dop.NoDiskOp?
       || (
-        && dop.RespReadSuperblockOp?
-        && !(s.LoadingSuperblock? && s.outstandingSuperblock1Read == Some(dop.id))
-        && !(s.LoadingSuperblock? && s.outstandingSuperblock2Read == Some(dop.id))
-      )
-      || (
-        && dop.RespReadJournalOp?
-        && !(s.LoadingOther? && s.journalFrontRead == Some(dop.id))
-        && !(s.LoadingOther? && s.journalBackRead == Some(dop.id))
-      )
-      || (
         && dop.RespReadIndirectionTableOp?
-        && !(s.LoadingOther? && s.indirectionTableRead == Some(dop.id))
+        && !(s.LoadingIndirectionTable? && s.indirectionTableRead == Some(dop.id))
       )
       || (
         && dop.RespReadNodeOp?
         && !(s.Ready? && dop.id in s.outstandingBlockReads)
-      )
-      || (
-        && dop.RespWriteSuperblockOp?
-        && !(s.Ready? && s.superblockWrite == Some(dop.id))
-      )
-      || (
-        && dop.RespWriteJournalOp?
-        && !(s.Ready? && dop.id in s.outstandingJournalWrites)
       )
       || (
         && dop.RespWriteIndirectionTableOp?
@@ -860,19 +376,9 @@ module BlockCache refines Transactable {
     && s'.outstandingBlockWrites == s.outstandingBlockWrites
     && s'.outstandingBlockReads == s.outstandingBlockReads
     && s'.frozenIndirectionTable == s.frozenIndirectionTable
-    && s'.syncReqs == s.syncReqs
 
     && s'.frozenIndirectionTableLoc == s.frozenIndirectionTableLoc
-    && s'.frozenJournalPosition == s.frozenJournalPosition
-    && s'.superblockWrite == s.superblockWrite
-    && s'.inMemoryJournal == s.inMemoryJournal
-    && s'.inMemoryJournalFrozen == s.inMemoryJournalFrozen
-    && s'.outstandingJournalWrites == s.outstandingJournalWrites
-    && s'.writtenJournalLen == s.writtenJournalLen
-    && s'.replayJournal == s.replayJournal
-    && s'.superblock == s.superblock
-    && s'.whichSuperblock == s.whichSuperblock
-    && s'.newSuperblock == s.newSuperblock
+    && s'.persistentIndirectionTableLoc == s.persistentIndirectionTableLoc
   }
 
   predicate Alloc(k: Constants, s: Variables, s': Variables, ref: Reference, block: Node)
@@ -897,19 +403,9 @@ module BlockCache refines Transactable {
     && s'.outstandingBlockWrites == s.outstandingBlockWrites
     && s'.outstandingBlockReads == s.outstandingBlockReads
     && s'.frozenIndirectionTable == s.frozenIndirectionTable
-    && s'.syncReqs == s.syncReqs
 
     && s'.frozenIndirectionTableLoc == s.frozenIndirectionTableLoc
-    && s'.frozenJournalPosition == s.frozenJournalPosition
-    && s'.superblockWrite == s.superblockWrite
-    && s'.inMemoryJournal == s.inMemoryJournal
-    && s'.inMemoryJournalFrozen == s.inMemoryJournalFrozen
-    && s'.outstandingJournalWrites == s.outstandingJournalWrites
-    && s'.writtenJournalLen == s.writtenJournalLen
-    && s'.replayJournal == s.replayJournal
-    && s'.superblock == s.superblock
-    && s'.whichSuperblock == s.whichSuperblock
-    && s'.newSuperblock == s.newSuperblock
+    && s'.persistentIndirectionTableLoc == s.persistentIndirectionTableLoc
   }
 
   predicate ReadStep(k: Constants, s: Variables, op: ReadOp)
@@ -925,73 +421,33 @@ module BlockCache refines Transactable {
     }
   }
 
-  predicate ValidJournalStep(s: Variables, js: JournalStep)
-  {
-    && s.Ready?
-    && (js.JSReplay? ==>
-      && IsPrefix(js.entries, s.replayJournal)
-    )
-    && (js.JSNew? ==>
-      && s.replayJournal == []
-    )
-  }
-
-  function DoJournalStep(s: Variables, js: JournalStep) : Variables
-  requires ValidJournalStep(s, js)
-  requires s.Ready?
-  {
-    match js {
-      case JSReplay(entries) =>
-        reveal_IsPrefix(); 
-        s.(replayJournal := s.replayJournal[|entries|..])
-      case JSNew(entries) =>
-        s.(inMemoryJournal := s.inMemoryJournal + entries)
-    }
-  }
-
-  predicate Transaction(k: Constants, s: Variables, s': Variables, dop: DiskOp, ops: seq<Op>, js: JournalStep)
+  predicate Transaction(k: Constants, s: Variables, s': Variables, dop: DiskOp, ops: seq<Op>)
   {
     && dop.NoDiskOp?
-
-    && ValidJournalStep(s, js)
-    && var s1 := DoJournalStep(s, js);
-
-    && OpTransaction(k, s1, s', ops)
+    && OpTransaction(k, s, s', ops)
   }
 
   predicate Init(k: Constants, s: Variables)
   {
-    s == LoadingSuperblock(None, None, SuperblockUnfinished, SuperblockUnfinished, map[])
+    s == Unready
   }
 
   predicate NextStep(k: Constants, s: Variables, s': Variables, dop: DiskOp, step: Step) {
     match step {
-      case WriteBackReqStep(ref) => WriteBackReq(k, s, s', dop, ref)
-      case WriteBackRespStep => WriteBackResp(k, s, s', dop)
+      case WriteBackNodeReqStep(ref) => WriteBackNodeReq(k, s, s', dop, ref)
+      case WriteBackNodeRespStep => WriteBackNodeResp(k, s, s', dop)
       case WriteBackIndirectionTableReqStep => WriteBackIndirectionTableReq(k, s, s', dop)
       case WriteBackIndirectionTableRespStep => WriteBackIndirectionTableResp(k, s, s', dop)
-      case WriteBackJournalReqStep(jr: JournalRange) => WriteBackJournalReq(k, s, s', dop, jr)
-      case WriteBackJournalRespStep => WriteBackJournalResp(k, s, s', dop)
-      case WriteBackSuperblockReq_Basic_Step => WriteBackSuperblockReq_Basic(k, s, s', dop)
-      case WriteBackSuperblockReq_UpdateIndirectionTable_Step => WriteBackSuperblockReq_UpdateIndirectionTable(k, s, s', dop)
-      case WriteBackSuperblockRespStep => WriteBackSuperblockResp(k, s, s', dop)
       case UnallocStep(ref) => Unalloc(k, s, s', dop, ref)
       case PageInReqStep(ref) => PageInReq(k, s, s', dop, ref)
       case PageInRespStep => PageInResp(k, s, s', dop)
       case PageInIndirectionTableReqStep => PageInIndirectionTableReq(k, s, s', dop)
       case PageInIndirectionTableRespStep => PageInIndirectionTableResp(k, s, s', dop)
-      case PageInJournalReqStep(which: int) => PageInJournalReq(k, s, s', dop, which)
-      case PageInJournalRespStep(which: int) => PageInJournalResp(k, s, s', dop, which)
-      case PageInSuperblockReqStep(which: int) => PageInSuperblockReq(k, s, s', dop, which)
-      case PageInSuperblockRespStep(which: int) => PageInSuperblockResp(k, s, s', dop, which)
-      case FinishLoadingSuperblockPhaseStep => FinishLoadingSuperblockPhase(k, s, s', dop)
-      case FinishLoadingOtherPhaseStep => FinishLoadingOtherPhase(k, s, s', dop)
+      case ReceiveLocStep => ReceiveLoc(k, s, s', dop)
       case EvictStep(ref) => Evict(k, s, s', dop, ref)
       case FreezeStep => Freeze(k, s, s', dop)
-      case PushSyncReqStep(id: uint64) => PushSyncReq(k, s, s', dop, id)
-      case PopSyncReqStep(id: uint64) => PopSyncReq(k, s, s', dop, id)
       case NoOpStep => NoOp(k, s, s', dop)
-      case TransactionStep(ops, js) => Transaction(k, s, s', dop, ops, js)
+      case TransactionStep(ops) => Transaction(k, s, s', dop, ops)
     }
   }
 
@@ -1069,37 +525,6 @@ module BlockCache refines Transactable {
         OutstandingBlockWritesDontOverlap(outstandingBlockWrites, id1, id2)
   }
 
-  predicate InvLoadingSuperblock(k: Constants, s: Variables)
-  requires s.LoadingSuperblock?
-  {
-    && (s.superblock1.SuperblockSuccess? ==>
-        && s.outstandingSuperblock1Read.None?
-        && WFSuperblock(s.superblock1.value)
-       )
-    && (s.superblock2.SuperblockSuccess? ==>
-        && s.outstandingSuperblock2Read.None?
-        && WFSuperblock(s.superblock2.value)
-       )
-    && (s.superblock1.SuperblockCorruption? ==>
-        && s.outstandingSuperblock1Read.None?
-        )
-    && (s.superblock2.SuperblockCorruption? ==>
-        && s.outstandingSuperblock2Read.None?
-        )
-  }
-
-  predicate InvLoadingOther(k: Constants, s: Variables)
-  requires s.LoadingOther?
-  {
-    && WFSuperblock(s.superblock)
-    && (s.indirectionTable.Some? ==>
-      && s.indirectionTableRead.None?
-      && WFCompleteIndirectionTable(s.indirectionTable.value)
-      && AllLocationsForDifferentRefsDontOverlap(s.indirectionTable.value)
-    )
-    && (s.whichSuperblock == 0 || s.whichSuperblock == 1)
-  }
-
   predicate InvReady(k: Constants, s: Variables)
   requires s.Ready?
   {
@@ -1114,19 +539,7 @@ module BlockCache refines Transactable {
     && OverlappingWritesEqForIndirectionTable(k, s, s.persistentIndirectionTable)
     && OutstandingWriteValidNodeLocation(s.outstandingBlockWrites)
     && AllOutstandingBlockWritesDontOverlap(s.outstandingBlockWrites)
-    && (s.superblockWrite.Some? <==> s.newSuperblock.Some?)
     && (s.frozenIndirectionTableLoc.Some? ==> s.frozenIndirectionTable.Some?)
-
-    && (s.whichSuperblock == 0 || s.whichSuperblock == 1)
-
-    && 0 <= s.writtenJournalLen <= NumJournalBlocks() as int
-    && 0 <= s.superblock.journalLen as int <= s.writtenJournalLen
-
-    && (s.frozenIndirectionTable.Some? ==> (
-      && 0 <= s.frozenJournalPosition <= NumJournalBlocks() as int
-      && s.superblock.journalLen as int <= s.writtenJournalLen
-      && s.frozenJournalPosition <= s.writtenJournalLen
-    ))
 
     // This isn't necessary for the other invariants in this file,
     // but it is useful for the implementation.
@@ -1146,51 +559,21 @@ module BlockCache refines Transactable {
       && WFCompleteIndirectionTable(s.frozenIndirectionTable.value)
     ))
 
-    && WFSuperblock(s.superblock)
-    && (s.newSuperblock.Some? ==>
-        && s.outstandingJournalWrites == {}
-
-        && (
-          || s.newSuperblock.value.indirectionTableLoc == s.superblock.indirectionTableLoc
-          || (
-            && s.frozenIndirectionTableLoc.Some?
-            && s.newSuperblock.value.indirectionTableLoc == s.frozenIndirectionTableLoc.value
-          )
-        )
-
-        && WFSuperblock(s.newSuperblock.value)
-        && s.newSuperblock.value.counter ==
-            IncrementSuperblockCounter(s.superblock.counter)
-        && s.inMemoryJournalFrozen == []
-        && (s.newSuperblock.value.indirectionTableLoc == s.superblock.indirectionTableLoc ==>
-            && s.newSuperblock.value.journalStart == s.superblock.journalStart
-            && s.newSuperblock.value.journalLen as int == s.writtenJournalLen
-        )
-        && (s.newSuperblock.value.indirectionTableLoc != s.superblock.indirectionTableLoc ==>
-            && s.outstandingIndirectionTableWrite.None?
-            && s.newSuperblock.value.journalStart as int == JournalPosAdd(s.superblock.journalStart as int, s.frozenJournalPosition)
-            && s.newSuperblock.value.journalLen as int == s.writtenJournalLen - s.frozenJournalPosition
-            && s.frozenJournalPosition as int + s.newSuperblock.value.journalLen as int
-                <= s.writtenJournalLen
-        )
-    )
+    && ValidIndirectionTableLocation(s.persistentIndirectionTableLoc)
     && (s.frozenIndirectionTableLoc.Some? ==> (
       && ValidIndirectionTableLocation(s.frozenIndirectionTableLoc.value)
       && !overlap(
           s.frozenIndirectionTableLoc.value,
-          s.superblock.indirectionTableLoc)
+          s.persistentIndirectionTableLoc)
     ))
-    && (s.inMemoryJournalFrozen != [] ==>
-      && s.frozenIndirectionTable.Some?
-      && s.frozenJournalPosition == s.writtenJournalLen
-    )
   }
 
   predicate Inv(k: Constants, s: Variables)
   {
-    && (s.LoadingSuperblock? ==> InvLoadingSuperblock(k, s))
-    && (s.LoadingOther? ==> InvLoadingOther(k, s))
     && (s.Ready? ==> InvReady(k, s))
+    && (s.LoadingIndirectionTable? ==>
+      ValidIndirectionTableLocation(s.indirectionTableLoc)
+    )
   }
 
   lemma InitImpliesInv(k: Constants, s: Variables)
@@ -1199,9 +582,9 @@ module BlockCache refines Transactable {
   {
   }
 
-  lemma WriteBackReqStepPreservesInv(k: Constants, s: Variables, s': Variables, dop: DiskOp, ref: Reference)
+  lemma WriteBackNodeReqStepPreservesInv(k: Constants, s: Variables, s': Variables, dop: DiskOp, ref: Reference)
     requires Inv(k, s)
-    requires WriteBackReq(k, s, s', dop, ref)
+    requires WriteBackNodeReq(k, s, s', dop, ref)
     ensures Inv(k, s')
   {
     if (s'.Ready?) {
@@ -1209,9 +592,9 @@ module BlockCache refines Transactable {
     }
   }
 
-  lemma WriteBackRespStepPreservesInv(k: Constants, s: Variables, s': Variables, dop: DiskOp)
+  lemma WriteBackNodeRespStepPreservesInv(k: Constants, s: Variables, s': Variables, dop: DiskOp)
     requires Inv(k, s)
-    requires WriteBackResp(k, s, s', dop)
+    requires WriteBackNodeResp(k, s, s', dop)
     ensures Inv(k, s')
   {
     if (s'.Ready?) {
@@ -1235,64 +618,6 @@ module BlockCache refines Transactable {
     ensures Inv(k, s')
   {
     if (s'.Ready?) {
-      assert InvReady(k, s');
-    }
-  }
-
-  lemma WriteBackJournalReqStepPreservesInv(k: Constants, s: Variables, s': Variables, dop: DiskOp, jr: JournalRange)
-    requires Inv(k, s)
-    requires WriteBackJournalReq(k, s, s', dop, jr)
-    ensures Inv(k, s')
-  {
-    if (s'.Ready?) {
-      assert InvReady(k, s');
-    }
-  }
-
-  lemma WriteBackJournalRespStepPreservesInv(k: Constants, s: Variables, s': Variables, dop: DiskOp)
-    requires Inv(k, s)
-    requires WriteBackJournalResp(k, s, s', dop)
-    ensures Inv(k, s')
-  {
-    if (s'.Ready?) {
-      assert InvReady(k, s');
-    }
-  }
-
-  lemma WriteBackSuperblockReq_Basic_StepPreservesInv(k: Constants, s: Variables, s': Variables, dop: DiskOp)
-    requires Inv(k, s)
-    requires WriteBackSuperblockReq_Basic(k, s, s', dop)
-    ensures Inv(k, s')
-  {
-    if (s'.Ready?) {
-      assert InvReady(k, s');
-    }
-  }
-
-  lemma WriteBackSuperblockReq_UpdateIndirectionTable_StepPreservesInv(k: Constants, s: Variables, s': Variables, dop: DiskOp)
-    requires Inv(k, s)
-    requires WriteBackSuperblockReq_UpdateIndirectionTable(k, s, s', dop)
-    ensures Inv(k, s')
-  {
-    if (s'.Ready?) {
-      assert InvReady(k, s');
-    }
-  }
-
-  lemma WriteBackSuperblockRespStepPreservesInv(k: Constants, s: Variables, s': Variables, dop: DiskOp)
-    requires Inv(k, s)
-    requires WriteBackSuperblockResp(k, s, s', dop)
-    ensures Inv(k, s')
-  {
-    if (s'.Ready?) {
-      /*if s'.frozenIndirectionTable.Some? {
-        if s.newSuperblock.value.indirectionTableLoc == s.superblock.indirectionTableLoc {
-          assert s'.superblock.journalLen as int <= s'.frozenJournalPosition;
-        } else {
-          assert s'.superblock.journalLen as int <= s'.frozenJournalPosition;
-        }
-      }*/
-
       assert InvReady(k, s');
     }
   }
@@ -1345,14 +670,13 @@ module BlockCache refines Transactable {
   }
 
 
-  lemma TransactionStepPreservesInv(k: Constants, s: Variables, s': Variables, dop: DiskOp, ops: seq<Op>, js: JournalStep)
+  lemma TransactionStepPreservesInv(k: Constants, s: Variables, s': Variables, dop: DiskOp, ops: seq<Op>)
     requires Inv(k, s)
-    requires Transaction(k, s, s', dop, ops, js)
+    requires Transaction(k, s, s', dop, ops)
     ensures Inv(k, s')
     decreases |ops|
   {
-    var s1 := DoJournalStep(s, js);
-    OpTransactionStepPreservesInv(k, s1, s', ops);
+    OpTransactionStepPreservesInv(k, s, s', ops);
   }
 
   lemma UnallocStepPreservesInv(k: Constants, s: Variables, s': Variables, dop: DiskOp, ref: Reference)
@@ -1405,59 +729,9 @@ module BlockCache refines Transactable {
     }
   }
 
-  lemma PageInJournalReqStepPreservesInv(k: Constants, s: Variables, s': Variables, dop: DiskOp, which: int)
+  lemma ReceiveLocStepPreservesInv(k: Constants, s: Variables, s': Variables, dop: DiskOp)
     requires Inv(k, s)
-    requires PageInJournalReq(k, s, s', dop, which)
-    ensures Inv(k, s')
-  {
-    if (s'.Ready?) {
-      assert InvReady(k, s');
-    }
-  }
-
-  lemma PageInJournalRespStepPreservesInv(k: Constants, s: Variables, s': Variables, dop: DiskOp, which: int)
-    requires Inv(k, s)
-    requires PageInJournalResp(k, s, s', dop, which)
-    ensures Inv(k, s')
-  {
-    if (s'.Ready?) {
-      assert InvReady(k, s');
-    }
-  }
-
-  lemma PageInSuperblockReqStepPreservesInv(k: Constants, s: Variables, s': Variables, dop: DiskOp, which: int)
-    requires Inv(k, s)
-    requires PageInSuperblockReq(k, s, s', dop, which)
-    ensures Inv(k, s')
-  {
-    if (s'.Ready?) {
-      assert InvReady(k, s');
-    }
-  }
-
-  lemma PageInSuperblockRespStepPreservesInv(k: Constants, s: Variables, s': Variables, dop: DiskOp, which: int)
-    requires Inv(k, s)
-    requires PageInSuperblockResp(k, s, s', dop, which)
-    ensures Inv(k, s')
-  {
-    if (s'.Ready?) {
-      assert InvReady(k, s');
-    }
-  }
-
-  lemma FinishLoadingSuperblockPhaseStepPreservesInv(k: Constants, s: Variables, s': Variables, dop: DiskOp)
-    requires Inv(k, s)
-    requires FinishLoadingSuperblockPhase(k, s, s', dop)
-    ensures Inv(k, s')
-  {
-    if (s'.Ready?) {
-      assert InvReady(k, s');
-    }
-  }
-
-  lemma FinishLoadingOtherPhaseStepPreservesInv(k: Constants, s: Variables, s': Variables, dop: DiskOp)
-    requires Inv(k, s)
-    requires FinishLoadingOtherPhase(k, s, s', dop)
+    requires ReceiveLoc(k, s, s', dop)
     ensures Inv(k, s')
   {
     if (s'.Ready?) {
@@ -1485,58 +759,26 @@ module BlockCache refines Transactable {
     }
   }
 
-  lemma PushSyncReqStepPreservesInv(k: Constants, s: Variables, s': Variables, dop: DiskOp, id: uint64)
-    requires Inv(k, s)
-    requires PushSyncReq(k, s, s', dop, id)
-    ensures Inv(k, s')
-  {
-    if (s'.Ready?) {
-      assert InvReady(k, s');
-    }
-  }
-
-  lemma PopSyncReqStepPreservesInv(k: Constants, s: Variables, s': Variables, dop: DiskOp, id: uint64)
-    requires Inv(k, s)
-    requires PopSyncReq(k, s, s', dop, id)
-    ensures Inv(k, s')
-  {
-    if (s'.Ready?) {
-      assert InvReady(k, s');
-    }
-  }
-
   lemma NextStepPreservesInv(k: Constants, s: Variables, s': Variables, dop: DiskOp, step: Step)
     requires Inv(k, s)
     requires NextStep(k, s, s', dop, step)
     ensures Inv(k, s')
   {
     match step {
-      case WriteBackReqStep(ref) => WriteBackReqStepPreservesInv(k, s, s', dop, ref);
-      case WriteBackRespStep => WriteBackRespStepPreservesInv(k, s, s', dop);
+      case WriteBackNodeReqStep(ref) => WriteBackNodeReqStepPreservesInv(k, s, s', dop, ref);
+      case WriteBackNodeRespStep => WriteBackNodeRespStepPreservesInv(k, s, s', dop);
       case WriteBackIndirectionTableReqStep => WriteBackIndirectionTableReqStepPreservesInv(k, s, s', dop);
       case WriteBackIndirectionTableRespStep => WriteBackIndirectionTableRespStepPreservesInv(k, s, s', dop);
-      case WriteBackJournalReqStep(jr: JournalRange) => WriteBackJournalReqStepPreservesInv(k, s, s', dop, jr);
-      case WriteBackJournalRespStep => WriteBackJournalRespStepPreservesInv(k, s, s', dop);
-      case WriteBackSuperblockReq_Basic_Step => WriteBackSuperblockReq_Basic_StepPreservesInv(k, s, s', dop);
-      case WriteBackSuperblockReq_UpdateIndirectionTable_Step => WriteBackSuperblockReq_UpdateIndirectionTable_StepPreservesInv(k, s, s', dop);
-      case WriteBackSuperblockRespStep => WriteBackSuperblockRespStepPreservesInv(k, s, s', dop);
       case UnallocStep(ref) => UnallocStepPreservesInv(k, s, s', dop, ref);
       case PageInReqStep(ref) => PageInReqStepPreservesInv(k, s, s', dop, ref);
       case PageInRespStep => PageInRespStepPreservesInv(k, s, s', dop);
       case PageInIndirectionTableReqStep => PageInIndirectionTableReqStepPreservesInv(k, s, s', dop);
       case PageInIndirectionTableRespStep => PageInIndirectionTableRespStepPreservesInv(k, s, s', dop);
-      case PageInJournalReqStep(which) => PageInJournalReqStepPreservesInv(k, s, s', dop, which);
-      case PageInJournalRespStep(which) => PageInJournalRespStepPreservesInv(k, s, s', dop, which);
-      case PageInSuperblockReqStep(which) => PageInSuperblockReqStepPreservesInv(k, s, s', dop, which);
-      case PageInSuperblockRespStep(which) => PageInSuperblockRespStepPreservesInv(k, s, s', dop, which);
-      case FinishLoadingSuperblockPhaseStep => FinishLoadingSuperblockPhaseStepPreservesInv(k, s, s', dop);
-      case FinishLoadingOtherPhaseStep => FinishLoadingOtherPhaseStepPreservesInv(k, s, s', dop);
+      case ReceiveLocStep => ReceiveLocStepPreservesInv(k, s, s', dop);
       case EvictStep(ref) => EvictStepPreservesInv(k, s, s', dop, ref);
       case FreezeStep => FreezeStepPreservesInv(k, s, s', dop);
-      case PushSyncReqStep(id) => PushSyncReqStepPreservesInv(k, s, s', dop, id);
-      case PopSyncReqStep(id) => PopSyncReqStepPreservesInv(k, s, s', dop, id);
       case NoOpStep => { }
-      case TransactionStep(ops, js) => TransactionStepPreservesInv(k, s, s', dop, ops, js);
+      case TransactionStep(ops) => TransactionStepPreservesInv(k, s, s', dop, ops);
     }
   }
 
