BlockCacheSystem/BlockDisk.i.dfy
@@ -1,0 +1,271 @@
+include "../MapSpec/MapSpec.s.dfy"
+include "../lib/Base/Maps.s.dfy"
+include "../PivotBetree/Bounds.i.dfy"
+include "DiskLayout.i.dfy"
+include "SectorType.i.dfy"
+include "AsyncSectorDiskModelTypes.i.dfy"
+
+//
+// An AsyncSectorDiskModel allows concurrent outstanding I/Os to a disk where each "sector"
+// is some higher-level Node datatype. A later refinement step shows how to marshall and align
+// these Nodes to the byte-ranges of the (trusted) AsyncDiskModel.
+//
+// TODO disallow concurrent spatially-overlapping writes/reads
+
+// A disk, processing stuff in its queue, doing its thing.
+module BlockDisk {
+  import opened NativeTypes
+  import opened Maps
+  import opened Options
+  import opened DiskLayout
+  import opened SectorType
+  import opened PivotBetreeGraph
+  import opened Sequences
+
+  type ReqId = uint64
+
+  datatype ReqReadIndirectionTable = ReqReadIndirectionTable(loc: Location)
+  datatype ReqReadNode = ReqReadNode(loc: Location)
+
+  datatype ReqWriteIndirectionTable = ReqWriteIndirectionTable(loc: Location, indirectionTable: IndirectionTable)
+  datatype ReqWriteNode = ReqWriteNode(loc: Location, node: Node)
+
+  datatype DiskOp =
+    | ReqReadIndirectionTableOp(id: ReqId, reqReadIndirectionTable: ReqReadIndirectionTable)
+    | ReqReadNodeOp(id: ReqId, reqReadNode: ReqReadNode)
+
+    | ReqWriteIndirectionTableOp(id: ReqId, reqWriteIndirectionTable: ReqWriteIndirectionTable)
+    | ReqWriteNodeOp(id: ReqId, reqWriteNode: ReqWriteNode)
+
+    | RespReadIndirectionTableOp(id: ReqId, indirectionTable: Option<IndirectionTable>)
+    | RespReadNodeOp(id: ReqId, node: Option<Node>)
+
+    | RespWriteIndirectionTableOp(id: ReqId)
+    | RespWriteNodeOp(id: ReqId)
+
+    | NoDiskOp
+
+  datatype Constants = Constants()
+  datatype Variables = Variables(
+    reqReadIndirectionTables: map<ReqId, ReqReadIndirectionTable>,
+    reqReadNodes: map<ReqId, ReqReadNode>,
+
+    reqWriteIndirectionTables: map<ReqId, Location>,
+    reqWriteNodes: map<ReqId, Location>,
+
+    // The disk:
+    indirectionTables: imap<Location, IndirectionTable>,
+    nodes: imap<Location, Node>
+  )
+
+  predicate Init(k: Constants, s: Variables)
+  {
+    && s.reqReadIndirectionTables == map[]
+    && s.reqReadNodes == map[]
+
+    && s.reqWriteIndirectionTables == map[]
+    && s.reqWriteNodes == map[]
+  }
+
+  ///////// RecvRead
+
+  predicate RecvReadIndirectionTable(k: Constants, s: Variables, s': Variables, dop: DiskOp)
+  {
+    && dop.ReqReadIndirectionTableOp?
+    && dop.id !in s.reqReadIndirectionTables
+    && s' == s.(reqReadIndirectionTables := s.reqReadIndirectionTables[dop.id := dop.reqReadIndirectionTable])
+  }
+
+  predicate RecvReadNode(k: Constants, s: Variables, s': Variables, dop: DiskOp)
+  {
+    && dop.ReqReadNodeOp?
+    && dop.id !in s.reqReadNodes
+    && s' == s.(reqReadNodes := s.reqReadNodes[dop.id := dop.reqReadNode])
+  }
+
+  ///////// RecvWrite
+
+  predicate DiskMapUpdate<T>(disk: imap<Location, T>, disk': imap<Location, T>, updateLoc: Location, t: T)
+  {
+    && updateLoc in disk'
+    && disk'[updateLoc] == t
+    && (forall loc | loc in disk && !overlap(loc, updateLoc) :: loc in disk' && disk'[loc] == disk[loc])
+    && (forall loc | loc in disk' && !overlap(loc, updateLoc) :: loc in disk)
+  }
+
+  predicate RecvWriteIndirectionTable(k: Constants, s: Variables, s': Variables, dop: DiskOp)
+  {
+    && dop.ReqWriteIndirectionTableOp?
+    && dop.id !in s.reqWriteIndirectionTables
+    && DiskMapUpdate(s.indirectionTables, s'.indirectionTables, dop.reqWriteIndirectionTable.loc, dop.reqWriteIndirectionTable.indirectionTable)
+    && s' == s.(reqWriteIndirectionTables := s.reqWriteIndirectionTables[dop.id := dop.reqWriteIndirectionTable.loc])
+              .(indirectionTables := s'.indirectionTables)
+  }
+
+  predicate RecvWriteNode(k: Constants, s: Variables, s': Variables, dop: DiskOp)
+  {
+    && dop.ReqWriteNodeOp?
+    && dop.id !in s.reqWriteNodes
+    && DiskMapUpdate(s.nodes, s'.nodes, dop.reqWriteNode.loc, dop.reqWriteNode.node)
+    && s' == s.(reqWriteNodes := s.reqWriteNodes[dop.id := dop.reqWriteNode.loc])
+              .(nodes := s'.nodes)
+  }
+
+  ///////// AckRead
+
+  predicate AckReadIndirectionTable(k: Constants, s: Variables, s': Variables, dop: DiskOp)
+  {
+    && dop.RespReadIndirectionTableOp?
+    && dop.id in s.reqReadIndirectionTables
+    && var req := s.reqReadIndirectionTables[dop.id];
+    && (dop.indirectionTable.Some? ==>
+      dop.indirectionTable == ImapLookupOption(s.indirectionTables, req.loc))
+    && s' == s.(reqReadIndirectionTables := MapRemove1(s.reqReadIndirectionTables, dop.id))
+  }
+
+  predicate AckReadNode(k: Constants, s: Variables, s': Variables, dop: DiskOp)
+  {
+    && dop.RespReadNodeOp?
+    && dop.id in s.reqReadNodes
+    && var req := s.reqReadNodes[dop.id];
+    && (dop.node.Some? ==>
+      dop.node == ImapLookupOption(s.nodes, req.loc))
+    && s' == s.(reqReadNodes := MapRemove1(s.reqReadNodes, dop.id))
+  }
+
+  ///////// AckWrite
+
+  predicate AckWriteIndirectionTable(k: Constants, s: Variables, s': Variables, dop: DiskOp)
+  {
+    && dop.RespWriteIndirectionTableOp?
+    && dop.id in s.reqWriteIndirectionTables
+    && s' == s.(reqWriteIndirectionTables := MapRemove1(s.reqWriteIndirectionTables, dop.id))
+  }
+
+  predicate AckWriteNode(k: Constants, s: Variables, s': Variables, dop: DiskOp)
+  {
+    && dop.RespWriteNodeOp?
+    && dop.id in s.reqWriteNodes
+    && s' == s.(reqWriteNodes := MapRemove1(s.reqWriteNodes, dop.id))
+  }
+
+  //// Stutter
+
+  predicate Stutter(k: Constants, s: Variables, s': Variables, dop: DiskOp)
+  {
+    && dop.NoDiskOp?
+    && s' == s
+  }
+
+  predicate Next(k: Constants, s: Variables, s': Variables, dop: DiskOp) {
+    && (dop.ReqReadIndirectionTableOp? ==> RecvReadIndirectionTable(k, s, s', dop))
+    && (dop.ReqReadNodeOp? ==> RecvReadNode(k, s, s', dop))
+
+    && (dop.ReqWriteIndirectionTableOp? ==> RecvWriteIndirectionTable(k, s, s', dop))
+    && (dop.ReqWriteNodeOp? ==> RecvWriteNode(k, s, s', dop))
+
+    && (dop.RespReadIndirectionTableOp? ==> AckReadIndirectionTable(k, s, s', dop))
+    && (dop.RespReadNodeOp? ==> AckReadNode(k, s, s', dop))
+
+    && (dop.RespWriteIndirectionTableOp? ==> AckWriteIndirectionTable(k, s, s', dop))
+    && (dop.RespWriteNodeOp? ==> AckWriteNode(k, s, s', dop))
+
+    && (dop.NoDiskOp? ==> Stutter(k, s, s', dop))
+  }
+
+  predicate UntouchedLoc(loc: Location, reqs: map<ReqId, Location>)
+  {
+    forall id | id in reqs :: !overlap(loc, reqs[id])
+  }
+
+  predicate havocMap<T>(
+    m: imap<Location, T>,
+    m': imap<Location, T>,
+    reqs: map<ReqId, Location>)
+  {
+    forall loc | loc in m ::
+        UntouchedLoc(loc, reqs) ==>
+            loc in m' && m'[loc] == m[loc]
+  }
+
+  predicate Crash(k: Constants, s: Variables, s': Variables)
+  {
+    && s.reqReadIndirectionTables == map[]
+    && s.reqReadNodes == map[]
+
+    && s.reqWriteIndirectionTables == map[]
+    && s.reqWriteNodes == map[]
+
+    && havocMap(s.indirectionTables, s'.indirectionTables, s.reqWriteIndirectionTables)
+    && havocMap(s.nodes, s'.nodes, s.reqWriteNodes)
+  }
+}
+
+abstract module BlockMachine {
+  import D = BlockDisk
+  import UI
+
+  type Variables
+  type Constants
+  type Location(==)
+  type Sector
+  type UIOp = UI.Op
+
+  predicate Init(k: Constants, s: Variables)
+  predicate Next(k: Constants, s: Variables, s': Variables, uiop: UIOp, dop: D.DiskOp)
+}
+
+// A disk attached to a program ("Machine"), modeling the nondeterministic crashes that reset the
+// program. Designed to look like the AsyncDiskModel, which we want to show refines to this.
+// TODO(jonh): Rename this to a "System"?
+abstract module BlockSystemModel {
+  import D = BlockDisk
+  import M : BlockMachine
+  import AsyncSectorDiskModelTypes
+  import opened SectorType
+
+  type Constants = AsyncSectorDiskModelTypes.AsyncSectorDiskModelConstants<M.Constants, D.Constants>
+  type Variables = AsyncSectorDiskModelTypes.AsyncSectorDiskModelVariables<M.Variables, D.Variables>
+  type UIOp = M.UIOp
+
+  datatype Step =
+    | MachineStep(dop: D.DiskOp)
+    | CrashStep
+  
+  predicate Machine(k: Constants, s: Variables, s': Variables, uiop: UIOp, dop: D.DiskOp)
+  {
+    && M.Next(k.machine, s.machine, s'.machine, uiop, dop)
+    && D.Next(k.disk, s.disk, s'.disk, dop)
+  }
+
+  predicate Crash(k: Constants, s: Variables, s': Variables, uiop: UIOp)
+  {
+    && uiop.CrashOp?
+    && M.Init(k.machine, s'.machine)
+    && D.Crash(k.disk, s.disk, s'.disk)
+  }
+
+  predicate NextStep(k: Constants, s: Variables, s': Variables, uiop: UIOp, step: Step)
+  {
+    match step {
+      case MachineStep(dop) => Machine(k, s, s', uiop, dop)
+      case CrashStep => Crash(k, s, s', uiop)
+    }
+  }
+
+  predicate Next(k: Constants, s: Variables, s': Variables, uiop: UIOp) {
+    exists step :: NextStep(k, s, s', uiop, step)
+  }
+
+  predicate Init(k: Constants, s: Variables)
+  predicate Inv(k: Constants, s: Variables)
+
+  lemma InitImpliesInv(k: Constants, s: Variables)
+    requires Init(k, s)
+    ensures Inv(k, s)
+
+  lemma NextPreservesInv(k: Constants, s: Variables, s': Variables, uiop: UIOp)
+    requires Inv(k, s)
+    requires Next(k, s, s', uiop)
+    ensures Inv(k, s')
+}
