MapSpec/FullVersioned.s.dfy
@@ -1,0 +1,109 @@
+include "../MapSpec/UIStateMachine.s.dfy"
+include "../lib/Base/Maps.s.dfy"
+//
+// Our definition of crash-safety.
+//
+
+abstract module FullVersioned {
+  import SM : UIStateMachine
+
+  import opened Maps
+  import UI
+
+  type Version = int
+  type SyncReqId = int
+
+  datatype Constants = Constants(k: SM.Constants)
+  datatype Variables = Variables(
+      ghost version: Version,
+      states: seq<SM.Variables>,
+      ghost syncReqs: map<SyncReqId, Version>
+  )
+
+  predicate Init(k: Constants, s: Variables)
+  {
+    && s.version == 0
+    && |s.states| == 1
+    && s.syncReqs == map[]
+  }
+
+  datatype Step =
+    | CrashStep
+    | AdvanceStep
+    | PersistStep
+    | PushSyncStep(ghost id: SyncReqId)
+    | PopSyncStep(ghost id: SyncReqId)
+    | StutterStep
+
+  predicate Crash(k: Constants, s: Variables, s': Variables, uiop: SM.UIOp)
+  {
+    && uiop.CrashOp?
+    && s'.version == 0
+    && |s.states| > 0
+    && s'.states == [s.states[0]]
+    && s'.syncReqs == map[]
+  }
+
+  predicate Advance(k: Constants, s: Variables, s': Variables, uiop: SM.UIOp)
+  {
+    && |s'.states| == |s.states| + 1
+    && |s.states| > 0
+    && s.states == s'.states[.. |s.states|]
+    && SM.Next(k.k,
+        s'.states[|s'.states| - 2],
+        s'.states[|s'.states| - 1],
+        uiop)
+    && s'.version == s.version
+    && s'.syncReqs == s.syncReqs
+  }
+
+  predicate Persist(k: Constants, s: Variables, s': Variables, uiop: SM.UIOp)
+  {
+    && uiop.NoOp?
+    && s.version <= s'.version <= s.version + |s.states| - 1
+    && s'.states == s.states[s'.version - s.version ..]
+    && s'.syncReqs == s.syncReqs
+  }
+
+  predicate PushSync(k: Constants, s: Variables, s': Variables, uiop: SM.UIOp, id: int)
+  {
+    && uiop == UI.PushSyncOp(id)
+    && id !in s.syncReqs
+    && s'.version == s.version
+    && s'.states == s.states
+    && s'.syncReqs ==
+        s.syncReqs[id := s.version + |s.states| - 1]
+  }
+
+  predicate PopSync(k: Constants, s: Variables, s': Variables, uiop: SM.UIOp, id: int)
+  {
+    && uiop == UI.PopSyncOp(id)
+    && id in s.syncReqs
+    && s.syncReqs[id] <= s.version
+    && s'.version == s.version
+    && s'.states == s.states
+    && s'.syncReqs == MapRemove1(s.syncReqs, id)
+  }
+
+  predicate Stutter(k: Constants, s: Variables, s': Variables, uiop: SM.UIOp)
+  {
+    && uiop.NoOp?
+    && s' == s
+  }
+
+  predicate NextStep(k: Constants, s: Variables, s': Variables, uiop: SM.UIOp, step: Step)
+  {
+    match step {
+      case CrashStep => Crash(k, s, s', uiop)
+      case AdvanceStep => Advance(k, s, s', uiop)
+      case PersistStep => Persist(k, s, s', uiop)
+      case PushSyncStep(id) => PushSync(k, s, s', uiop, id)
+      case PopSyncStep(id) => PopSync(k, s, s', uiop, id)
+      case StutterStep => Stutter(k, s, s', uiop)
+    }
+  }
+
+  predicate Next(k: Constants, s: Variables, s': Variables, uiop: SM.UIOp) {
+    exists step :: NextStep(k, s, s', uiop, step)
+  }
+}
